Challenge/Modexp/Submission/Proofs/Memo/PCs/T21.lean
@@ -7,9 +7,9 @@ namespace Challenge.Modexp.Submission.Proofs.Memo.PCs
 
 open Challenge.Modexp.Submission.Proofs.Bytecode
 
-@[simp] theorem pc21 (i : Nat) (hlo : 1712 ≤ i) (hhi : i ≤ 1731) :
+@[simp] theorem pc21 (i : Nat) (hlo : 1712 ≤ i) (hhi : i ≤ 1734) :
     Artifact.submissionArtifact.instructionPC i =
-      [4139,4141,4142,4175,4177,4178,4211,4213,4214,4247,4249,4250,4283,4285,4286,4319,4321,4322,4325,4326][i - 1712]! := by
+      [4103,4105,4106,4139,4141,4142,4175,4177,4178,4211,4213,4214,4247,4249,4250,4283,4285,4286,4319,4321,4322,4325,4326][i - 1712]! := by
   interval_cases i <;> decide +kernel
 
 end Challenge.Modexp.Submission.Proofs.Memo.PCs
