Challenge/Modexp/Submission/Proofs/Memo/V3/Paths.lean
@@ -17,46 +17,31 @@ def preludePath :
     List (Challenge.EvmProof.Stepper.Located Artifact.submissionArtifact .Osaka) :=
   [
    Main.opAt 1142 (EvmSemantics.Operation.StackMemFlow (EvmSemantics.Operation.StackMemFlowOps.JUMPDEST)),
-   Main.pushAt 1143 1 1,
-   Main.pushAt 1144 0 0,
+   Main.pushAt 1143 30 290062066191873733550822415321244206417662036842114019324193742671314944,
+   Main.pushAt 1144 1 94,
    Main.opAt 1145 (EvmSemantics.Operation.Env (EvmSemantics.Operation.EnvOps.CALLDATALOAD)),
    Main.opAt 1146 (EvmSemantics.Operation.CompBit (EvmSemantics.Operation.CompareBitwiseOps.XOR))
-  ]
-
-def chunk0Path :
-    List (Challenge.EvmProof.Stepper.Located Artifact.submissionArtifact .Osaka) :=
-  [
-   Main.pushAt 1147 1 1,
-   Main.pushAt 1148 1 32,
-   Main.opAt 1149 (EvmSemantics.Operation.Env (EvmSemantics.Operation.EnvOps.CALLDATALOAD)),
-   Main.opAt 1150 (EvmSemantics.Operation.CompBit (EvmSemantics.Operation.CompareBitwiseOps.XOR)),
-   Main.opAt 1151 (EvmSemantics.Operation.CompBit (EvmSemantics.Operation.CompareBitwiseOps.OR)),
-   Main.pushAt 1152 30 290062066191873733550822415321244206417662036842114019324193742671314944,
-   Main.pushAt 1153 1 94,
-   Main.opAt 1154 (EvmSemantics.Operation.Env (EvmSemantics.Operation.EnvOps.CALLDATALOAD)),
-   Main.opAt 1155 (EvmSemantics.Operation.CompBit (EvmSemantics.Operation.CompareBitwiseOps.XOR)),
-   Main.opAt 1156 (EvmSemantics.Operation.CompBit (EvmSemantics.Operation.CompareBitwiseOps.OR))
   ]
 
 def branchPath :
     List (Challenge.EvmProof.Stepper.Located Artifact.submissionArtifact .Osaka) :=
   [
-   Main.pushAt 1157 2 1196,
-   Main.opAt 1158 (EvmSemantics.Operation.StackMemFlow (EvmSemantics.Operation.StackMemFlowOps.JUMPI))
+   Main.pushAt 1147 2 1196,
+   Main.opAt 1148 (EvmSemantics.Operation.StackMemFlow (EvmSemantics.Operation.StackMemFlowOps.JUMPI))
   ]
 
 def branchPrefixPath :
     List (Challenge.EvmProof.Stepper.Located Artifact.submissionArtifact .Osaka) :=
   [
-   Main.pushAt 1157 2 1196
+   Main.pushAt 1147 2 1196
   ]
 
 def returnPath :
     List (Challenge.EvmProof.Stepper.Located Artifact.submissionArtifact .Osaka) :=
   [
-   Main.pushAt 1159 0 0,
-   Main.pushAt 1160 0 0,
-   Main.opAt 1161 (EvmSemantics.Operation.System (EvmSemantics.Operation.SystemOps.RETURN))
+   Main.pushAt 1149 0 0,
+   Main.pushAt 1150 0 0,
+   Main.opAt 1151 (EvmSemantics.Operation.System (EvmSemantics.Operation.SystemOps.RETURN))
   ]
 
 end Challenge.Modexp.Submission.Proofs.Memo.V3.Paths
